{"nbformat":4,"nbformat_minor":0,"metadata":{"colab":{"provenance":[],"authorship_tag":"ABX9TyPiOXKJFuRegi1WoW7MzIKU"},"kernelspec":{"name":"python3","display_name":"Python 3"},"language_info":{"name":"python"}},"cells":[{"cell_type":"markdown","source":["3 a)\n","\n","$\\theta_{MAP}=\\arg\\max_\\theta p(\\theta|x,y)=\\arg\\max_\\theta p(\\theta,x,y)$ and $\\arg\\max_\\theta p(y|x,\\theta)p(\\theta|x)=\\arg\\max_\\theta p(y,x,\\theta)/p(x,\\theta)\\cdot p(\\theta, x)/p(x)=\\arg\\max_\\theta p(x,y,\\theta)/p(x)=\\arg\\max_\\theta p(x,y,\\theta)$. So, $\\theta_{MAP}=\\arg\\max_\\theta p(y|x,\\theta)p(\\theta)$.\n","\n","3 b)\n","\n","$\\arg\\max_\\theta p(y|x,\\theta)\\frac{1}{(2\\pi)^{k/2}|\\Sigma|^{1/2}} \\exp(-\\frac{1}{2}\\theta^T\\Sigma^{-1}\\theta)=\\arg\\max_\\theta p(y|x,\\theta)\\frac{1}{(2\\pi)^{k/2}\\eta^k} \\exp(-\\frac{\\eta^{-2}}{2}\\sum_{i=1}^k\\theta_i^2)=\\arg\\max_\\theta \\log( p(y|x,\\theta)\\frac{1}{(2\\pi)^{k/2}\\eta^k} \\exp(-\\frac{\\eta^{-2}}{2}\\sum_{i=1}^k\\theta_i^2)=\\arg\\max_\\theta \\log p(y|x,\\theta)-\\frac{\\eta^{-2}}{2}\\sum_{i=1}^k\\theta_i^2=\\arg\\min_\\theta -\\log p(y|x,\\theta)+\\frac{\\eta^{-2}}{2}||\\theta||_2^2$. So, the value of $\\lambda$ is $\\eta^{-2}/2$.\n","\n","3 c)\n","\n","$\\theta_{MAP}=\\arg\\min_\\theta -\\sum_{i=1}^m \\log p(y_i|x_i,\\theta)+\\frac{\\eta^{-2}}{2}||\\theta||_2^2$\n","\n","$=\\arg\\min_{\\theta}-\\sum_{i=1}^m \\log(\\exp(-(y_i-\\theta^T x_i)^2/(2\\sigma^2)))+\\frac{\\eta^{-2}}{2}||\\theta||_2^2$\n","\n","$=\\arg\\min_\\theta \\sum_{i=1}^m (y_i-\\theta^T x_i)^2/(2\\sigma^2)+\\frac{\\eta^{-2}}{2}||\\theta||_2^2$\n","\n","$=\\arg\\min_\\theta \\frac{1}{2\\sigma^2}(Y-X\\theta)^T(Y-X \\theta)+\\frac{\\eta^{-2}}{2}||\\theta||_2^2$.\n","\n","Since $f(\\theta)=\\frac{1}{2\\sigma^2}(Y-X\\theta)_i(Y-X \\theta)^i+\\frac{\\eta^{-2}}{2}\\theta_i\\theta^i$ is convex, $\\nabla f(\\theta)=0$ gives the optimal $\\theta$. $\\nabla f(\\theta)_k=\\frac{1}{2\\sigma^2}(-X_{ik})(Y-X\\theta)^i+\\frac{1}{2\\sigma^2}(Y-X\\theta)_i(-X)_{ik}+\\eta^{-2}\\theta_k=-\\frac{1}{\\sigma^2}(Y-X\\theta)^TX+\\eta^{-2}\\theta$. So $\\nabla f(\\theta)=0$ iff $\\eta^{-2}\\theta=\\frac{1}{\\sigma^2}X^T(Y-X\\theta)$ iff $\\eta^{-2}\\theta=\\frac{1}{\\sigma^2}X^T Y-\\frac{1}{\\sigma^2}X^TX\\theta$ iff $\\theta=(\\eta^{-2} I+\\frac{1}{\\sigma^2}X^TX)^{-1}\\frac{1}{\\sigma^2}X^TY=(\\sigma^2\\eta^{-2} I+X^TX)^{-1}X^TY$.\n","\n","3 d)\n","\n","$\\theta_{MAP}=\\arg\\max_\\theta p(y|x,\\theta)p(\\theta)=\\arg\\max_\\theta \\log (p(y|x,\\theta))+\\log p(\\theta)=\\arg\\max_\\theta \\log(exp(-(y-x^T\\theta)^2/(2\\sigma^2)))+\\log(\\exp((-|\\theta|/b))=\\arg\\max_\\theta (-(y-x^T\\theta)^2/(2\\sigma^2))-|\\theta|/b=\\arg\\min_\\theta(y-x^T\\theta)^2/(2\\sigma^2)+|\\theta|/b=\\arg\\min_\\theta||X\\theta-Y||_2^2+\\frac{2\\sigma^2}{b}|\\theta|$. So, $\\gamma=\\frac{2\\sigma^2}{b}$.\n","\n","\n","\n"],"metadata":{"id":"CYTYW1BZhENH"}}]}