{"nbformat":4,"nbformat_minor":0,"metadata":{"colab":{"provenance":[],"authorship_tag":"ABX9TyOYDxiS1ohkMi1l/XZ22GCs"},"kernelspec":{"name":"python3","display_name":"Python 3"},"language_info":{"name":"python"}},"cells":[{"cell_type":"markdown","source":["5 a)\n","\n","$||B(V_1)-B(V_2)||_\\infty$$=||\\gamma\\max_{a\\in A}\\sum_{s'\\in S}P_{sa}(s')V_1(s')-\\gamma\\max_{a\\in A}\\sum_{s'\\in S}P_{sa}(s')V_2(s')||_\\infty$$=\\gamma||\\max_{a\\in A}\\sum_{s'\\in S}P_{sa}(s')(V_1(s')-V_2(s'))||_\\infty$$\\leq\\gamma||V_1(s')-V_2(s')||_\\infty$.\n","\n","5 b)\n","\n","Suppose there are $2$ fixed points $V_1$ and $V_2$, then $B(V_1)=V_1$ and $B(V_2)=V_2$. $||B(V_1)-B(V_2)||_\\infty=||V_1-V_2||_\\infty$. So, $||V_1-V_2||_\\infty\\leq \\gamma||V_1-V_2||_\\infty$. So, $||V_1-V_2||_\\infty=0$. So, $V_1=V_2$."],"metadata":{"id":"TsndkiNZaMYJ"}}]}