{"nbformat":4,"nbformat_minor":0,"metadata":{"colab":{"provenance":[],"authorship_tag":"ABX9TyMAxMiPagP/LKu6agPf0ICF"},"kernelspec":{"name":"python3","display_name":"Python 3"},"language_info":{"name":"python"}},"cells":[{"cell_type":"markdown","source":["3\n","\n","\n","$f_u(x)$$=\\arg\\min_{v=\\alpha u}||x-v||^2$$=x \\cdot u u$. $||x^{(i)}-f_u(x^{(i)})||_2^2$$=||x^{(i)}-x^{(i)}\\cdot u u||^2_2$$=(x^{(i)}-x^{(i)}\\cdot u u)\\cdot (x^{(i)}-x^{(i)}\\cdot u u)$$=x^{(i)}\\cdot x^{(i)}-2(x^{(i)}\\cdot u)^2+(x^{(i)}\\cdot u)^2(u\\cdot u)$$=x^{(i)}\\cdot x^{(i)}-(x^{(i)}\\cdot u)^2$. So, $\\arg\\min_u \\sum_{i=1}^m||x^{(i)}-f_u(x^{(i)})||_2^2$$=\\arg\\min_u\\sum_{i=1}^m-(x^{(i)}\\cdot u)^2$$=\\arg\\max_u\\sum_{i=1}^m (x^{(i)}\\cdot u)^2$, which is the first principal component."],"metadata":{"id":"YnW32sH_H_ui"}}]}