{"nbformat":4,"nbformat_minor":0,"metadata":{"colab":{"provenance":[],"authorship_tag":"ABX9TyPowaODB1TzOM90hN1wmCtp"},"kernelspec":{"name":"python3","display_name":"Python 3"},"language_info":{"name":"python"}},"cells":[{"cell_type":"markdown","source":["2 a)\n","$D_{KL}(P,Q)=E_P[\\log(\\frac{P(x)}{Q(x)})]$$=E_P[-\\log (\\frac{Q(x)}{P(x)})]$$\\geq -\\log E_P[\\frac{Q(x)}{P(x)}]$$=-\\log\\sum_{x\\in X}Q(x)=0$ with the inequality standing iff $\\frac{Q(x)}{P(x)}=E_P[\\frac{Q(x)}{P(x)}]=1$.\n","\n","2 b)\n","$D_{KL}(P(X,Y)||Q(X,Y))$$=\\sum_{(x,y)}P(x,y)\\log (\\frac{P(x,y)}{Q(x,y)})$$=\\sum_{(x,y)}(P(x,y)(\\log (\\frac{P(y|x)}{Q(y|x)})+\\log(\\frac{P(x)}{Q(x)})))$$=\\sum_x(P(x)\\log(\\frac{P(x)}{Q(x)}))+\\sum_x\\sum_y(P(x,y)\\log (\\frac{P(y|x)}{Q(y|x)}))$$=\\sum_x (P(x)\\log(\\frac{P(x)}{Q(x)}))+\\sum_xP(x)\\sum_y(P(y|x)\\log (\\frac{P(y|x)}{Q(y|x)}))$$=D_{KL}(P(X)||Q(X))+D_{KL}(P(Y|X)||Q(Y|X))$\n","\n","2 c)\n","$RHS$$=\\arg\\max_\\theta m\\sum_x\\hat{P}(x)\\log(P_\\theta (x)) $$=\\arg\\max_\\theta \\sum_x \\hat{P}(x)\\log(P_\\theta(x))$$=\\arg\\min_\\theta\\sum_x \\hat{P}(x)\\log(\\hat{P}(x))-\\sum_x\\hat{P}(x)\\log(P_\\theta(x))$$=\\arg\\min_\\theta \\sum_x (\\hat{P}(x)\\log(\\frac{\\hat{P}(x)}{P_\\theta(x)}))=LHS$"],"metadata":{"id":"OCS2nek3CeF9"}}]}