{"nbformat":4,"nbformat_minor":0,"metadata":{"colab":{"provenance":[],"authorship_tag":"ABX9TyM7Mu1pPKjElT9DyBgtJSAq"},"kernelspec":{"name":"python3","display_name":"Python 3"},"language_info":{"name":"python"}},"cells":[{"cell_type":"markdown","source":["4 a)\n","\n","$E[Y|X,\\theta]=\\int_{\\mathbb{R}}y b(y)exp(\\eta y-a(\\eta))dy$.\n","\n","$\\frac{\\partial}{\\partial\\eta}p(y;\\eta)=(y-a'(\\eta))p(y;\\eta)$.\n","\n","$\\frac{\\partial}{\\partial\\eta}\\int p(y;\\eta)dy=\\frac{\\partial}{\\partial\\eta} 1=0$.\n","\n","$\\int (y-a'(\\eta))p(y;\\eta)dy=0$.\n","\n","So, $E[Y|X;\\theta]=\\int a'(\\eta)p(y;\\eta)dy=a'(\\eta)$.\n","\n","\n","4b)\n","\n","$var(Y|X;\\theta)=E[Y^2|X;\\theta]-E[Y|X;\\theta]^2$.\n","\n","$E[Y^2|X;\\theta]=\\int y^2 p(y;\\eta)dy$\n","\n","$\\frac{\\partial^2}{\\partial\\eta^2}p(y;\\eta)=\\frac{\\partial}{\\partial\\eta}(y-a'(\\eta))p(y;\\eta)=\\frac{\\partial}{\\partial\\eta}yp(y;\\eta)-\\frac{\\partial}{\\partial\\eta}a'(\\eta)p(y;\\eta)=y(y-a'(\\eta))p(y;\\eta)-a''(\\eta)p(y;\\eta)-a'(\\eta)(y-a'(\\eta))p(y;\\eta)=y^2p(y;\\eta)-2ya'(\\eta)p(y;\\eta)+a'(\\eta)^2p(y;\\eta)-a''(\\eta)p(y;\\eta)$.\n","\n","$\\int\\frac{\\partial^2}{\\partial\\eta^2}p(y;\\eta)dy=\\frac{\\partial^2}{\\partial\\eta^2}\\int p(y;\\eta)dy=0$.\n","\n","$\\int y^2p(y;\\eta)-2ya'(\\eta)p(y;\\eta)+a'(\\eta)^2p(y;\\eta)-a''(\\eta)p(y;\\eta)dy=0$.\n","\n","$E[Y^2|X;\\theta]=\\int y^2p(y;\\eta)dy=\\int 2ya'(\\eta)p(y;\\eta)-a'(\\eta)^2p(y;\\eta)+a''(\\eta)p(y;\\eta)dy=2a'(\\eta)E[Y|X;\\theta]-a'(\\eta)^2+a''(\\eta)=a'(\\eta)^2+a''(\\eta)$.\n","\n","$var(Y|X;\\theta)=E[Y^2|X;\\theta]-E[Y|X;\\theta]^2=a'(\\eta)^2+a''(\\eta)-a'(\\eta)^2=a''(\\eta)$.\n","\n","\n","4c)\n","\n","$l(\\theta)=\\log L(\\theta)=\\log p(y|x;\\theta)=\\log b(y)+\\eta y-a(\\eta)$.\n","\n","$NLL=-l(\\theta)=-\\log b(y)-\\eta y+a(\\eta)=-\\log b(y)-\\theta^T x y+a(\\theta^T x)$.\n","\n","$\\frac{\\partial}{\\partial\\theta}NLL=\\frac{\\partial\\eta}{\\partial\\theta}\\frac{\\partial NLL}{\\partial \\eta}=x\\frac{\\partial NLL}{\\partial\\eta}=-x(y-a'(\\eta))$.\n","\n","$\\nabla^2_\\theta NLL_{ij}=\\partial(-x_i(y-a'(\\eta)))/\\partial \\theta_j=x_ix_ja''(\\eta)$.\n","\n","Since $a''(\\eta)=var(Y|X;\\theta)\\geq 0$, $\\nabla^2_\\theta NLL$ is PSD."],"metadata":{"id":"cl4vO2PzCuig"}}]}